src/Mail2/MailServer.v
@@ -1,7 +1,11 @@
 Require Import POCS.
-Require Import String.
 Require Import MailServerAPI.
-Require Import FMapFacts.
+
+Require Import MailServerDirAPI.
+Require Import MailServerDirImpl.
+
+Require Import MailboxAPI.
+Require Import MailboxImpl.
 
 
 Import MailServerAPI.
@@ -19,3 +23,16 @@ Definition do_mail_req : proc opT unit :=
 
 Definition mail_server_thread : proc MailServerAPI.opT unit :=
   Until (fun _ => false) (fun _ => do_mail_req) tt.
+
+Definition mail_server :=
+  repeat (Proc mail_server_thread) 4.
+
+
+Module c := Link MailboxAPI MailServerDirAPI MailServerAPI
+                 AtomicReader MailServerDir.
+
+
+Definition ms_bottom := c.compile_ts mail_server.
+Check ms_bottom.
+
+Print Assumptions c.compile_traces_match.
