src/Mail2/MailServerDirImpl.v
@@ -1,0 +1,59 @@
+Require Import POCS.
+Require Import MailServerAPI.
+Require Import MailServerDirAPI.
+
+
+Module MailServerDir <: LayerImpl MailServerDirAPI MailServerAPI.
+
+  Definition absR (s1 : MailServerDirAPI.State) (s2 : MailServerAPI.State) :=
+    FMap.is_permutation_val (FSet.elements s2) s1.
+
+  Definition compile_ts (ts : @threads_state MailServerAPI.opT) := ts.
+
+  Theorem compile_ts_no_atomics :
+    forall (ts : @threads_state MailServerAPI.opT),
+      no_atomics_ts ts ->
+      no_atomics_ts (compile_ts ts).
+  Proof.
+    unfold compile_ts; eauto.
+  Qed.
+
+  Theorem absR_ok :
+    op_abs absR MailServerDirAPI.step MailServerAPI.step.
+  Proof.
+    unfold op_abs; intros.
+(*
+    destruct s1; inversion H; clear H.
+    simpl in *; subst.
+    unfold absR.
+    destruct op; inversion H0; clear H0; repeat sigT_eq.
+    all: eexists; intuition eauto; constructor.
+  Qed.
+*)
+  Admitted.
+
+  Hint Resolve absR_ok.
+
+  Theorem compile_traces_match :
+    forall ts,
+      no_atomics_ts ts ->
+      traces_match_abs absR
+        MailServerDirAPI.initP MailServerDirAPI.step
+        MailServerAPI.step (compile_ts ts) ts.
+  Proof.
+    unfold compile_ts, traces_match_abs; intros.
+    eexists; intuition idtac.
+    eapply trace_incl_abs; eauto.
+    eauto.
+  Qed.
+
+  Theorem absInitP :
+    forall s1 s2,
+      MailServerDirAPI.initP s1 ->
+      absR s1 s2 ->
+      MailServerAPI.initP s2.
+  Proof.
+    eauto.
+  Qed.
+
+End MailServerDir.
